SimplePCFa: termination lemmas and substVXs for ECIU

proof/DDC/Language/SimplePCFa/EquivCIU.v
@@ -1,35 +1,70 @@
 
+Require Export DDC.Language.SimplePCFa.ExpSubsts.
 Require Export DDC.Language.SimplePCFa.TyJudge.
 Require Export DDC.Language.SimplePCFa.Step.
+Require Export DDC.Language.SimplePCFa.Eval.
 Require DDC.Base.
 
 
-(* Expressions are ciu-equivalent at the given type. *)
-Definition ECIU (x1 x2 : exp) (t: ty)
- := TYPEX nil x1 t 
- /\ TYPEX nil x2 t
- /\ (forall f, TERMF f x1 <-> TERMF f x2).
+(* Expressions are ciu-equivalent at the given type
+   c.i.u = closed instantiation of use.
+   For two open terms, 
+     when we substitution any sets of closing values into them,
+     then the terminatinon behavior of the two terms is the same
+     in all contexts (the use)
+*)
+Definition EQCIU (te: tyenv) (x1 x2: exp) (t: ty)
+ := forall te x1 x2 t
+ ,  TYPEX te x1 t
+ -> TYPEX te x2 t
+ -> (forall f vs x1' x2'
+      ,  Forall2 (fun v => TYPEX nil (XVal v)) vs te    
+      -> csubstVXs vs x1 x1'
+      -> csubstVXs vs x2 x2'
+      -> (TERMF f x1' <-> TERMF f x2')).
 
 
-Lemma ecui_if_true
- :  forall x x1 x2 t
- ,  x = XIf (VConst (CBool true)) x1 x2
- -> TYPEX nil x    t
- -> ECIU      x x1 t.
+Lemma eqciu_from_eval
+ :  forall te x1 x2 t
+ ,  TYPEX te x1 t
+ -> TYPEX te x2 t
+ -> (    (exists x1', EVAL x1 x1') 
+     <-> (exists x2', EVAL x2 x2') )
+ -> EQCIU te x1 x2 t.
 Proof.
- intros. subst.
- red. rip. inverts H0. burn.
-
- split.
-  intros.
-  inverts H.
-  inverts H1. auto.
-
-  intros. eauto.
+ intros.
+ red. rip.
+ split; intros;
+  eapply eval_term_wrapped; eauto.
 Qed.
 
 
+Lemma eqciu_from_eval'
+ :  forall te x1 x2 t
+ ,  TYPEX te x1 t
+ -> TYPEX te x2 t 
+ -> (forall f, (exists x3, EVAL (wrap f x1) x3) 
+           <-> (exists x4, EVAL (wrap f x2) x4))
+ -> EQCIU te x1 x2 t.
+Proof.
+ intros.
+ red. rip.
+ admit.         (* TODO *)
+Qed.
 
+
+Lemma eqciu_if_true
+ :  forall te x x1 x2 t
+ ,  x = XIf (VConst (CBool true)) x1 x2
+ -> TYPEX te x    t
+ -> EQCIU te x x1 t.
+Proof.
+ intros. subst.
+ red. rip. inverts H0. burn.
+Qed.
+
+
+(*
 (* TODO: finish me, lower indices (S i) to i *)
 Definition lowerXX (d: nat) (x: exp) : exp
  := x.
@@ -45,7 +80,7 @@ Lemma eciu_if_let_let_nest
  -> wfX 0 x2 
               (* TODO: and x3 doesn't ref x2 *)
  -> TYPEX nil z1 t3
- -> ECIU  z1  z2 t3.
+ -> EQCIU  z1  z2 t3.
 Proof.
  admit.  (* TODO *)
 Qed.
@@ -64,7 +99,7 @@ Lemma ecui_if_let_let_swap
  -> z2 = XLet t2 (lowerXX 0 x2) (XLet t1 (liftXX 0 x1) (swapXX 0 x3))
  -> wfX 0 x2
  -> TYPEX nil z1 t3
- -> ECIU  z1  z2 t3.
+ -> EQCIU  z1  z2 t3.
 Proof.
  intros. subst.
  red. rip.
@@ -79,4 +114,4 @@ Proof.
  admit.
 Qed.
 
-
+*)
