proof/DDC/Language/SimplePCFa.v
@@ -3,6 +3,7 @@
 Require Export DDC.Language.SimplePCFa.Exp.
 Require Export DDC.Language.SimplePCFa.ExpLift.
 Require Export DDC.Language.SimplePCFa.ExpSubst.
+Require Export DDC.Language.SimplePCFa.ExpSubsts.
 
 (* Type Expressions *)
 Require Export DDC.Language.SimplePCFa.Ty.
@@ -17,6 +18,9 @@ Require Export DDC.Language.SimplePCF.SubstExpExp.
 (* Small step evaluation. *)
 Require Export DDC.Language.SimplePCFa.Step.
 
+(* Big step evaluation, and conversion between small step evaluation. *)
+Require Export DDC.Language.SimplePCFa.Eval.
+
 (*
 (* A well typed expression is either a value or can take a step. *)
 Require Export DDC.Language.SimplePCF.Progress.
@@ -24,6 +28,4 @@ Require Export DDC.Language.SimplePCF.Progress.
 (* When an expression takes a step then the result has the same type. *)
 Require Export DDC.Language.SimplePCF.Preservation.
 
-(* Big step evaluation, and conversion between small step evaluation. *)
-Require Export DDC.Language.SimplePCF.Eval.
 *)
